wip

Garden/Brevis/chips/gadgets/add.v
@@ -26,12 +26,12 @@ Module AddGadget.
   }.
 
   Definition eval {p} `{Prime p}
-      (a b : Array.t Z 4)
+      (a b : Word.t)
       (cols : t)
       (is_real : Z) :
       M.t unit :=
     let one := 1 in
-    let base := 256 mod p in
+    let base := 256 in
 
     let* _ := M.when is_real (
       let overflow_0 := a.[0] +F b.[0] -F cols.(value).[0] in
@@ -39,30 +39,200 @@ Module AddGadget.
       let overflow_2 := a.[2] +F b.[2] -F cols.(value).[2] +F cols.(carry).[1] in
       let overflow_3 := a.[3] +F b.[3] -F cols.(value).[3] +F cols.(carry).[2] in
 
-      let* _ := M.assert_zero (overflow_0 *F (overflow_0 -F base)) in
-      let* _ := M.assert_zero (overflow_1 *F (overflow_1 -F base)) in
-      let* _ := M.assert_zero (overflow_2 *F (overflow_2 -F base)) in
-      let* _ := M.assert_zero (overflow_3 *F (overflow_3 -F base)) in
+      let* _ := M.assert_either_zero overflow_0 (overflow_0 -F base) in
+      let* _ := M.assert_either_zero overflow_1 (overflow_1 -F base) in
+      let* _ := M.assert_either_zero overflow_2 (overflow_2 -F base) in
+      let* _ := M.assert_either_zero overflow_3 (overflow_3 -F base) in
 
-      let* _ := M.assert_zero (cols.(carry).[0] *F (overflow_0 -F base)) in
-      let* _ := M.assert_zero (cols.(carry).[1] *F (overflow_1 -F base)) in
-      let* _ := M.assert_zero (cols.(carry).[2] *F (overflow_2 -F base)) in
+      (* let* _ := M.assert_either_zero cols.(carry).[0] (overflow_0 -F base) in
+      let* _ := M.assert_either_zero cols.(carry).[1] (overflow_1 -F base) in
+      let* _ := M.assert_either_zero cols.(carry).[2] (overflow_2 -F base) in *)
 
-      let* _ := M.assert_zero ((cols.(carry).[0] -F one) *F overflow_0) in
-      let* _ := M.assert_zero ((cols.(carry).[1] -F one) *F overflow_1) in
-      let* _ := M.assert_zero ((cols.(carry).[2] -F one) *F overflow_2) in
+      (* let* _ := M.assert_either_zero (cols.(carry).[0] -F one) overflow_0 in
+      let* _ := M.assert_either_zero (cols.(carry).[1] -F one) overflow_1 in
+      let* _ := M.assert_either_zero (cols.(carry).[2] -F one) overflow_2 in
 
       let* _ := M.assert_bool cols.(carry).[0] in
       let* _ := M.assert_bool cols.(carry).[1] in
       let* _ := M.assert_bool cols.(carry).[2] in
-      let* _ := M.assert_bool is_real in
+      let* _ := M.assert_bool is_real in *)
 
       M.Pure tt
     ) in
-    let* _ :=
+    (* let* _ :=
       let* _ := slice_range_check_u8 a is_real in
       let* _ := slice_range_check_u8 b is_real in
       let* _ := slice_range_check_u8 cols.(value) is_real in
-      M.pure tt in
+      M.pure tt in *)
     M.Pure tt.
+
+  Module ForEachN.
+    Fixpoint t_nat (N : nat) (P : Z -> Prop) : Prop :=
+      match N with
+      | O => True
+      | S N => P (Z.of_nat N) /\ t_nat N P
+      end.
+
+    Definition t (N : Z) (P : Z -> Prop) : Prop :=
+      t_nat (Z.to_nat N) P.
+
+    Lemma implies_forall_nat (N : nat) (P : Z -> Prop)
+        (H_P : t_nat N P) :
+      forall i, 0 <= i < Z.of_nat N ->
+      P i.
+    Proof.
+      induction N; cbn in *; intros.
+      { lia. }
+      { assert (0 <= i < Z.of_nat N \/ i = Z.of_nat N) as [] by lia.
+        all: best.
+      }
+    Qed.
+
+    Lemma implies_forall (N : Z) (P : Z -> Prop)
+      (H_P : ForEachN.t N P) :
+      forall i, 0 <= i < N ->
+      P i.
+    Proof.
+      assert (N < 0 \/ N = Z.of_nat (Z.to_nat N)) as [? | H_N] by lia.
+      { lia. }
+      { rewrite H_N.
+        now apply implies_forall_nat.
+      }
+    Qed.
+  End ForEachN.
+
+  Lemma eval_correct {p} `{Prime p} (H_p : 2 ^ 9 < p)
+      (a' b' : Z)
+      (cols' : t)
+      (* (is_real : bool) *)
+      (H_a : 0 <= a' < 2 ^ 32)
+      (H_b : 0 <= b' < 2 ^ 32) :
+    let a := Word.of_Z a' in
+    let b := Word.of_Z b' in
+    let cols := M.map_mod cols' in
+    let is_real := Z.b2z true in
+    {{ eval a b cols is_real 🔽
+      tt,
+      cols.(value) =F Word.of_Z (a' + b')
+    }}.
+  Proof.
+    unfold eval.
+    eapply Run.Implies. {
+      Run.run.
+    }
+    intros H_post.
+    destruct H_post as [H_post _].
+    epose proof (H_post ltac:(cbn; lia)) as H_post'; clear H_post.
+    cbn in *; unfold Pos.to_nat in *; cbn in *.
+    set (col0 := UnOp.from cols'.(value) .[ 0]) in *.
+    set (col1 := UnOp.from cols'.(value) .[ 1]) in *.
+    set (col2 := UnOp.from cols'.(value) .[ 2]) in *.
+    set (col3 := UnOp.from cols'.(value) .[ 3]) in *.
+    set (carry0 := cols'.(carry).[0]) in *.
+    set (carry1 := cols'.(carry).[1]) in *.
+    set (carry2 := cols'.(carry).[2]) in *.
+    assert (0 <= col0 < 2 ^ 8) by admit.
+    assert (0 <= col1 < 2 ^ 8) by admit.
+    assert (0 <= col2 < 2 ^ 8) by admit.
+    assert (0 <= col3 < 2 ^ 8) by admit.
+    (* assert (0 <= carry0 < 2) by admit.
+    assert (0 <= carry1 < 2) by admit.
+    assert (0 <= carry2 < 2) by admit. *)
+    apply ForEachN.implies_forall.
+    repeat constructor.
+    all: cbn; unfold Pos.to_nat; cbn.
+    all: fold col0 col1 col2 col3.
+    all: unfold BinOp.add, BinOp.sub in *.
+    all: assert (H_foo : forall z, z mod p = z) by admit.
+    all: repeat rewrite H_foo in * |-; clear H_foo.
+    Time 4: lia.
+    Time 3: lia.
+    4: {
+      repeat destruct H_post' as [? H_post'].
+      replace carry0 with 0 in * by admit.
+      replace carry1 with 0 in * by admit.
+      replace carry2 with 0 in * by admit.
+      Time lia.
+      repeat match goal with
+      | H : _ |- _ => clear H
+      end.
+      lia.
+      destruct H_post' as [? _].
+      lia.
+    }
+    Time 4: lia.
+    all: lia.
+
+    Search List.seq.
+    intros i. 
+    rewrite <- List.in_seq.
+    clearbody col0 col1 col2 col3 carry0 carry1 carry2.
+    repeat rewrite M.mul_zero_implies_zero in *.
+    autorewrite with field_rewrite in *.
+    unfold UnOp.from in *.
+    rewrite (M.from_small carry0) in * by (clear H_post'; lia).
+    rewrite (M.from_small carry1) in * by (clear H_post'; lia).
+    rewrite (M.from_small carry2) in * by (clear H_post'; lia).
+    unfold BinOp.add, BinOp.sub in *.
+    assert (H_foo : forall z, z mod p = z) by admit.
+    repeat rewrite H_foo in * |-.
+    clear H_foo.
+    intros.
+    replace i with 3 by admit.
+    replace (cols'.(value) .[ 3] mod p) with col3 by admit.
+    cbn; unfold Pos.to_nat; cbn.
+    Time lia.
+    replace i with 0 by admit.
+    replace (cols'.(value) .[ 0] mod p) with col0 by admit.
+    cbn; unfold Pos.to_nat; cbn.
+    Time lia.
+    replace i with 1 by admit.
+    replace (cols'.(value) .[ 1] mod p) with col1 by admit.
+    cbn; unfold Pos.to_nat; cbn.
+    Time lia.
+    replace i with 2 by admit.
+    replace (cols'.(value) .[ 2] mod p) with col2 by admit.
+    cbn; unfold Pos.to_nat; cbn.
+    Time lia.
+    repeat (match goal with | H : _ /\ _ |- _ => destruct H end).
+    rewrite M.mul_zero_implies_zero in *.
+    autorewrite with field_rewrite in *.
+    rewrite M.sub_zero_equiv in *.
+    destruct H2 as [H2|H2].
+    {
+      assert (0 <= UnOp.from cols'.(value) .[ 0] < 2 ^ 8) by admit.
+    assert (UnOp.from cols'.(value) .[ 0] <)
+    intros.
+    replace i with 0 by admit.
+    cbn.
+    repeat (match goal with | H : _ /\ _ |- _ => destruct H end).
+    rewrite M.mul_zero_implies_zero in *.
+    autorewrite with field_rewrite in *.
+    rewrite M.sub_zero_equiv in *.
+    destruct H2 as [H2|H2].
+    {
+      assert (0 <= UnOp.from cols'.(value) .[ 0] < 2 ^ 8) by admit.
+      rewrite <- H2 in *.
+      autorewrite with field_rewrite in *.
+      unfold "+F" in *.
+      revert H_p H21; clear; intros.
+      rewrite Z.mod_small in * by lia.
+      lia.
+    }
+    {
+      assert (0 <= UnOp.from cols'.(value) .[ 0] < 2 ^ 8) by admit.
+      assert (a' mod 256 +F b' mod 256 -F 256 mod p = cols'.(value) .[ 0]) by admit.
+      rewrite <- H22 in *.
+      revert H_p H21; clear; intros.
+      autorewrite with field_rewrite in *.
+      unfold "+F", BinOp.sub in *.
+      repeat rewrite M.from_small in * by lia.
+      rewrite (M.from_small 256) in * by lia.
+      lia.
+    }
+    {
+
+    }
+    intuition.
+  Qed.
 End AddGadget.
