Garden/Brevis/compiler/riscv/opcode.v
@@ -1,5 +1,89 @@
 Require Import Garden.Plonky3.M.
 
+Module Opcode.
+  Inductive t : Set :=
+  | ADD
+  | SUB
+  | XOR
+  | OR
+  | AND
+  | SLL
+  | SRL
+  | SRA
+  | SLT
+  | SLTU
+  | LB
+  | LH
+  | LW
+  | LBU
+  | LHU
+  | SB
+  | SH
+  | SW
+  | BEQ
+  | BNE
+  | BLT
+  | BGE
+  | BLTU
+  | BGEU
+  | JAL
+  | JALR
+  | AUIPC
+  | ECALL
+  | EBREAK
+  | MUL
+  | MULH
+  | MULHU
+  | MULHSU
+  | DIV
+  | DIVU
+  | REM
+  | REMU
+  | UNIMP.
+
+  Definition to_Z (self : t) : Z :=
+    match self with
+    | ADD => 0
+    | SUB => 1
+    | XOR => 2
+    | OR => 3
+    | AND => 4
+    | SLL => 5
+    | SRL => 6
+    | SRA => 7
+    | SLT => 8
+    | SLTU => 9
+    | LB => 10
+    | LH => 11
+    | LW => 12
+    | LBU => 13
+    | LHU => 14
+    | SB => 15
+    | SH => 16
+    | SW => 17
+    | BEQ => 18
+    | BNE => 19
+    | BLT => 20
+    | BGE => 21
+    | BLTU => 22
+    | BGEU => 23
+    | JAL => 24
+    | JALR => 25
+    | AUIPC => 27
+    | ECALL => 28
+    | EBREAK => 29
+    | MUL => 30
+    | MULH => 31
+    | MULHU => 32
+    | MULHSU => 33
+    | DIV => 34
+    | DIVU => 35
+    | REM => 36
+    | REMU => 37
+    | UNIMP => 39
+    end.
+End Opcode.
+
 Module ByteOpcode.
   Inductive t : Set :=
   | AND
