Garden/Brevis/compiler/word.v
@@ -9,6 +9,29 @@ Module Word.
     map_mod x := M.map_mod x;
   }.
 
-  Global Instance IsGenerate : MGenerate.C t :=
-    _.
+  Global Instance IsGenerate : MGenerate.C t := _.
+
+  Global Instance IsEqual : Equal.C t := {
+    Equal.t x y := x =F y;
+  }.
+
+  Definition of_Z (z : Z) : t :=
+    Array.of_list [
+      z mod 256;
+      (z / 256) mod 256;
+      (z / 256 / 256) mod 256;
+      (z / 256 / 256 / 256) mod 256
+    ].
+
+  (** We do not use field arithmetic there, as this function is only for specifications. *)
+  Definition to_Z (self : t) : Z :=
+    self.[0] + 256 * (self.[1] + 256 * (self.[2] + 256 * self.[3])).
+
+  Lemma to_Z_of_Z (z : Z) (H_z : 0 <= z < 2 ^ 32) :
+    to_Z (of_Z z) = z.
+  Proof.
+    unfold of_Z, to_Z.
+    cbv - [Z.add Z.mul Z.div Z.modulo].
+    lia.
+  Qed.
 End Word.
