Garden/Brevis/chips/chips/alu/add_sub/constraints.v
@@ -1,0 +1,36 @@
+Require Import Garden.Plonky3.M.
+Require Import Garden.Brevis.chips.chips.alu.add_sub.columns.
+Require Import Garden.Brevis.chips.gadgets.add.
+Require Import Garden.Brevis.compiler.riscv.opcode.
+Require Import Garden.Brevis.machine.builder.lookup.
+
+Definition eval {p} `{Prime p} (local : AddSubCols.t) : M.t unit :=
+  M.for_each local.(AddSubCols.values) (fun value =>
+    let '{|
+      AddSubValueCols.add_operation := add_operation;
+      AddSubValueCols.operand_1 := operand_1;
+      AddSubValueCols.operand_2 := operand_2;
+      AddSubValueCols.is_add := is_add;
+      AddSubValueCols.is_sub := is_sub;
+    |} := value in
+    let* _ := AddGadget.eval operand_1 operand_2 add_operation (is_add +F is_sub) in
+
+    let opcode := is_add *F Opcode.to_Z Opcode.ADD
+        +F is_sub *F Opcode.to_Z Opcode.SUB in
+
+    let* _ :=
+      looked_alu
+        opcode
+        add_operation.(AddGadget.value)
+        operand_1
+        operand_2
+        is_add in
+
+    let* _ := looked_alu opcode operand_1 add_operation.(AddGadget.value) operand_2 is_sub in
+
+    let is_real := is_add +F is_sub in
+    let* _ := M.assert_bool is_add in
+    let* _ := M.assert_bool is_sub in
+    let* _ := M.assert_bool is_real in
+    M.pure tt
+  ).
