Garden/Brevis/machine/builder/lookup.v
@@ -1,7 +1,27 @@
 Require Import Garden.Plonky3.M.
 Require Import Garden.Brevis.M.
 Require Import Garden.Brevis.compiler.riscv.opcode.
+Require Import Garden.Brevis.compiler.word.
 Require Import Garden.Brevis.machine.lookup.
+
+Definition looked_alu
+    (opcode : Z)
+    (a : Word.t)
+    (b : Word.t)
+    (c : Word.t)
+    (multiplicity : Z) :
+    M.t unit :=
+  let values :=
+    [opcode] ++
+    Array.to_list a ++
+    Array.to_list b ++
+    Array.to_list c in
+  looked {|
+    SymbolicLookup.values := values;
+    SymbolicLookup.multiplicity := multiplicity;
+    SymbolicLookup.kind := LookupType.Alu;
+    SymbolicLookup.scope := LookupScope.Regional;
+  |}.
 
 Definition looking_byte_pair
     (opcode : Z)
